Saturn/Solverstep.lean
@@ -1,6 +1,7 @@
 import Saturn.FinSeq
 import Saturn.Clause 
 open Nat
+open Vector
 
 def boundOpt(n: Nat) : Option (Nat) → Prop
   | none => True
@@ -56,42 +57,43 @@ theorem mapPlusOneShift{n : Option Nat}{m : Nat} : n.map (. + 1) = some (m + 1) 
     congrArg some lem2
 
 structure RestrictionClauses{dom n: Nat}(branch: Bool)(focus: Nat)(focusLt : focus < n + 1)
-    (clauses: FinSeq dom (Clause (n + 1))) where
+    (clauses: Vector (Clause (n + 1)) dom) where
   codom : Nat
-  restClauses : FinSeq codom  (Clause n)
+  restClauses : Vector  (Clause n) codom
   forward : (k: Nat) → k < dom → Option Nat
   forwardWit : (k: Nat) → (w: k < dom) → boundOpt codom (forward k w)
   reverse : (k : Nat) → (k < codom) → Nat
   reverseWit : (k : Nat) → (w : k < codom) → reverse k w < dom
   
 structure DroppedProof{dom n: Nat}{branch: Bool}{focus: Nat}{focusLt : focus < n + 1}
-    {clauses: FinSeq dom (Clause (n + 1))}(
+    {clauses: Vector (Clause (n + 1)) dom}(
         rc: RestrictionClauses branch focus focusLt clauses)  where
     dropped : (k : Nat) → (w: k < dom) → rc.forward k w = 
-        none → (clauses k w focus focusLt = some branch)
+        none → (Vector.at (clauses.at k w) focus focusLt = some branch)
 
 structure ForwardRelation{dom n: Nat}{branch: Bool}{focus: Nat}{focusLt : focus < n + 1}
-    {clauses: FinSeq dom (Clause (n + 1))}(
+    {clauses: Vector (Clause (n + 1)) dom}(
         rc: RestrictionClauses branch focus focusLt clauses)  where
     forwardRelation : (k : Nat) → (w: k < dom) → (j: Nat) →  rc.forward k w = some j →
-    (jw : j < rc.codom) →  delete focus focusLt (clauses k w) = 
-      rc.restClauses j jw
+    (jw : j < rc.codom) →  delete focus focusLt (Vector.at (clauses.at k w)) = 
+      Vector.at (rc.restClauses.at j jw)
 
 structure ReverseRelation{dom n: Nat}{branch: Bool}{focus: Nat}{focusLt : focus < n + 1}
-    {clauses: FinSeq dom (Clause (n + 1))}(
+    {clauses: Vector (Clause (n + 1)) dom}(
         rc: RestrictionClauses branch focus focusLt clauses)  where
     relation : (k : Nat) → (w: k < rc.codom) → 
-      rc.restClauses k w = delete focus focusLt 
-        (clauses (rc.reverse k w) (rc.reverseWit k w))
+      Vector.at (rc.restClauses.at k w) = delete focus focusLt 
+        (Vector.at (clauses.at (rc.reverse k w) (rc.reverseWit k w)))
 
 structure NonPosReverse{dom n: Nat}{branch: Bool}{focus: Nat}{focusLt : focus < n + 1}
-    {clauses: FinSeq dom (Clause (n + 1))}(
+    {clauses: Vector (Clause (n + 1)) dom}(
         rc: RestrictionClauses branch focus focusLt clauses)  where
     nonPosRev : (k : Nat) → (w: k < rc.codom)  → 
-      Not ((clauses (rc.reverse k w) (rc.reverseWit k w)) focus focusLt = some branch)
+      Not (
+        Vector.at (clauses.at (rc.reverse k w) (rc.reverseWit k w)) focus focusLt = some branch)
 
 structure RestrictionData{dom n: Nat}(branch: Bool)(focus: Nat)(focusLt : focus < n + 1)
-    (clauses: FinSeq dom (Clause (n + 1))) where
+    (clauses: Vector (Clause (n + 1)) dom) where
     restrictionClauses : RestrictionClauses branch focus focusLt clauses
     droppedProof : DroppedProof restrictionClauses
     forwardRelation : ForwardRelation restrictionClauses
@@ -100,29 +102,38 @@ structure RestrictionData{dom n: Nat}(branch: Bool)(focus: Nat)(focusLt : focus 
 
 
 def pullBackSolution{dom n: Nat}(branch: Bool)(focus : Nat)(focusLt : focus < n + 1)
-    (clauses: FinSeq dom (Clause (n + 1)))(rc: RestrictionClauses branch focus focusLt clauses) 
+    (clauses: Vector (Clause (n + 1)) dom)(rc: RestrictionClauses branch focus focusLt clauses) 
     (dp : DroppedProof rc) (fr: ForwardRelation rc): 
       (valuation : Valuation n) → 
-        ((j : Nat) → (jw : j < rc.codom) → ClauseSat (rc.restClauses j jw) valuation) → 
+        ((j : Nat) → (jw : j < rc.codom) → ClauseSat (rc.restClauses.at j jw) valuation) → 
         (j : Nat) → (jw : j < dom) →  
-          ClauseSat (clauses j jw) (insert branch n focus focusLt valuation) := 
+          ClauseSat (clauses.at j jw) (FinSeq.vec (insert branch n focus focusLt valuation.at)) := 
         fun valuation pf =>
           fun k w => 
             let splitter := optCase (rc.forward k w)
             match splitter with
             | OptCase.noneCase eqn => 
-              let lem1 : clauses k w focus focusLt = some branch := dp.dropped k w eqn
-              let lem2 : insert branch n focus focusLt valuation focus focusLt = branch := by 
+              let lem1 : Vector.at (clauses.at k w) focus focusLt = some branch := dp.dropped k w eqn
+              let lem2 : insert branch n focus focusLt valuation.at focus focusLt = branch := by 
                 apply insertAtFocus
                 done
-              let lem3 : clauses k w focus focusLt = 
-                some (insert branch n focus focusLt valuation focus focusLt) := 
+              let lem3 : Vector.at (clauses.at k w) focus focusLt = 
+                some (insert branch n focus focusLt valuation.at focus focusLt) := 
                 by
                   rw lem1
                   apply (congrArg some)
                   exact Eq.symm lem2
                   done
-              ⟨focus, focusLt, lem3⟩
+              let lem4 : (Vector.at (Vector.at clauses k w) focus focusLt) = some (
+                  (Vector.at 
+                    (FinSeq.vec (insert branch n focus focusLt 
+                      (Vector.at valuation))) focus focusLt)) := 
+                      by 
+                        rw (seqAt (insert branch n focus focusLt 
+                      (Vector.at valuation)))
+                        rw lem3
+                        done
+              ⟨focus, focusLt, lem4⟩
             | OptCase.someCase j eqn => 
               let bound := rc.forwardWit k w 
               let jWitAux : boundOpt rc.codom (some j) := by
@@ -132,43 +143,65 @@ def pullBackSolution{dom n: Nat}(branch: Bool)(focus : Nat)(focusLt : focus < n 
               let jWit : j < rc.codom := jWitAux
               let lem1 := fr.forwardRelation k w j eqn jWit
               let ⟨i, iw, vs⟩ := pf j jWit
-              let lem2 : rc.restClauses j jWit i iw = some (valuation i iw) := vs
-              let lem3 : delete focus focusLt (clauses k w) i iw =
-                  some (valuation i iw) := 
+              let lem2 : Vector.at (rc.restClauses.at j jWit) i iw = 
+                      some (valuation.at i iw) := vs
+              let lem3 : delete focus focusLt (Vector.at (clauses.at k w)) i iw =
+                  some (valuation.at i iw) := 
                     by
                     rw (Eq.symm lem2)
                     rw lem1
                     done
-              let lem4 : delete focus focusLt (clauses k w) i iw =
-                clauses k w (skip focus i) (skipPlusOne iw) := by
+              let lem4 : delete focus focusLt (Vector.at (clauses.at k w)) i iw =
+                (Vector.at (clauses.at k w)) (skip focus i) (skipPlusOne iw) := by
                   rfl
                   done
-              let lem5 : insert branch n focus focusLt valuation 
+              let lem5 : insert branch n focus focusLt valuation.at 
                               (skip focus i) (skipPlusOne iw) =
-                                  valuation i iw := by
+                                  valuation.at i iw := by
                                     apply insertAtImage
                                     done
-              let lem6 : clauses k w (skip focus i) (skipPlusOne iw) =
-                          some (insert branch n focus focusLt valuation 
+              let lem6 : (Vector.at (clauses.at k w)) (skip focus i) (skipPlusOne iw) =
+                          some (insert branch n focus focusLt valuation.at 
                               (skip focus i) (skipPlusOne iw)) := by
                               rw (Eq.symm lem4)
                               rw lem3
                               rw lem5
                               done
-              ⟨skip focus i, skipPlusOne iw, lem6⟩
+              let lem7 : (Vector.at (Vector.at clauses k w) (skip focus i) (skipPlusOne iw)) =
+                some (
+                  (Vector.at (FinSeq.vec (insert branch n focus focusLt (Vector.at valuation))) 
+                    (skip focus i) (skipPlusOne iw))) := 
+                      by
+                        rw (seqAt (insert branch n focus focusLt (Vector.at valuation)))
+                        rw lem6
+                        done
+              ⟨skip focus i, skipPlusOne iw, lem7⟩
 
 
 def unitClause(n : Nat)(b : Bool)(k : Nat) (w : k < n + 1):   Clause (n + 1):=
-  insert (some b) n k w (contradiction n) 
+  FinSeq.vec (insert (some b) n k w (Vector.at (contradiction n))) 
 
 theorem unitDiag(n : Nat)(b : Bool)(k : Nat) (w : k < n + 1): 
-          unitClause n b k w k w = b :=
-          insertAtFocus (some b) n k w (contradiction n)
+          Vector.at (unitClause n b k w) k w = b := by
+            have resolve  : unitClause n b k w = 
+                FinSeq.vec (insert (some b) n k w (Vector.at (contradiction n))) := rfl
+            rw resolve
+            rw seqAt
+            apply insertAtFocus (some b) n k w (Vector.at (contradiction n))
+            done
 
 theorem unitSkip(n : Nat)(b : Bool)(k : Nat) (w : k < n + 1): 
-          (i: Nat) → (iw : i < n) →  unitClause n b k w (skip k i) 
-                  (skipPlusOne iw) = none := fun i iw => 
-          insertAtImage (some b) n k w (contradiction n) i iw
+          (i: Nat) → (iw : i < n) →  Vector.at (unitClause n b k w) (skip k i) 
+                  (skipPlusOne iw) = none := by 
+                  intros i iw
+                  have resolve  : unitClause n b k w = 
+                        FinSeq.vec (insert (some b) n k w (Vector.at (contradiction n))) := rfl
+                  rw resolve
+                  rw seqAt 
+                  let ins := insertAtImage (some b) n k w (Vector.at (contradiction n)) i iw
+                  rw ins
+                  rw contraAt
+                  done
 
 structure IsUnitClause{n: Nat}(clause: Clause (n +1)) where
   index: Nat 
@@ -179,14 +212,14 @@ structure IsUnitClause{n: Nat}(clause: Clause (n +1)) where
 def clauseUnit{n: Nat}(clause: Clause (n + 1)) : Option (IsUnitClause clause) :=
   let f : Fin (n + 1) →   (Option (IsUnitClause clause)) := 
     fun ⟨k, w⟩ =>
-      match deqSeq _ clause  (unitClause n true k w) with 
+      match deqSeq _ clause.at (Vector.at (unitClause n true k w)) with 
       | isTrue pf => 
-        let cl : IsUnitClause clause := IsUnitClause.mk k w true pf 
+        let cl : IsUnitClause clause := IsUnitClause.mk k w true (equalCoords pf) 
         some (cl)
       | isFalse _ => 
-        match deqSeq _ clause  (unitClause n false k w) with 
+        match deqSeq _ clause.at (Vector.at (unitClause n false k w)) with 
       | isTrue pf => 
-        let cl : IsUnitClause clause := IsUnitClause.mk k w false pf 
+        let cl : IsUnitClause clause := IsUnitClause.mk k w false (equalCoords pf) 
         some (cl)
       | isFalse _ => none  
   let seq : FinSeq (n + 1) (Fin (n + 1)) := fun k w => ⟨k, w⟩
@@ -223,29 +256,32 @@ def someUnitClause {l : Nat} {n : Nat}: (clauses : FinSeq l  (Clause (n + 1))) �
     fun clauses =>
      someUnitClauseAux clauses l (Nat.leRefl l) none
 
-structure HasPureVar{dom n : Nat}(clauses : FinSeq dom  (Clause n)) where
+structure HasPureVar{dom n : Nat}(clauses : Vector  (Clause n) dom) where
   index : Nat
   bound : index < n
   parity : Bool
   evidence : (k : Nat) → (lt : k < dom) → 
-          (clauses k lt index bound = none) ∨  (clauses k lt index bound = some parity)
+          (Vector.at (clauses.at k lt) index bound = none) ∨  
+            (Vector.at (clauses.at k lt) index bound = some parity)
 
-structure IsPureVar{dom n : Nat}(clauses : FinSeq dom  (Clause n))
+structure IsPureVar{dom n : Nat}(clauses : Vector  (Clause n) dom) 
                       (index: Nat)(bound : index < n)(parity : Bool) where
-  evidence : (k : Nat) → (lt : k < dom) → (clauses k lt index bound = none) ∨ 
-                                (clauses k lt index bound = some parity)
+  evidence : (k : Nat) → (lt : k < dom) → (Vector.at (clauses.at k lt) index bound = none) ∨ 
+                                (Vector.at (clauses.at k lt) index bound = some parity)
 
-def pureEvidence {dom n : Nat}(clauses : FinSeq dom  (Clause n)) 
+def pureEvidence {dom n : Nat}(clauses : Vector  (Clause n) dom) 
                   (index: Nat)(bound : index < n)(parity : Bool): Prop := 
                   (k : Nat) → (lt : k < dom) → 
-          (clauses k lt index bound = none) ∨  (clauses k lt index bound = some parity)
+          (Vector.at (clauses.at k lt) index bound = none) ∨  
+          (Vector.at (clauses.at k lt) index bound = some parity)
 
-def pureBeyond{dom n : Nat}(clauses : FinSeq dom  (Clause n)) 
+def pureBeyond{dom n : Nat}(clauses : Vector  (Clause n) dom) 
                   (index: Nat)(bound : index < n)(parity : Bool)(m: Nat): Prop := 
                   (k : Nat) → (lt : k < dom) → (m ≤ k) → 
-          (clauses k lt index bound = none) ∨  (clauses k lt index bound = some parity)
+          (Vector.at (clauses.at k lt) index bound = none) ∨  
+          (Vector.at (clauses.at k lt) index bound = some parity)
 
-def pureBeyondZero{dom n : Nat}(clauses : FinSeq dom  (Clause n))
+def pureBeyondZero{dom n : Nat}(clauses : Vector  (Clause n) dom)
                 (index: Nat)(bound : index < n)(parity : Bool) : 
                   pureBeyond clauses index bound parity 0 → 
                   pureEvidence clauses index bound parity := by
@@ -255,7 +291,7 @@ def pureBeyondZero{dom n : Nat}(clauses : FinSeq dom  (Clause n))
                     exact hyp k kw  (Nat.zeroLe k)
                     done   
 
-def pureBeyondVacuous{dom n : Nat}(clauses : FinSeq dom  (Clause n))
+def pureBeyondVacuous{dom n : Nat}(clauses : Vector  (Clause n) dom)
             (index: Nat)(bound : index < n)(parity : Bool)(m: Nat)(le: dom ≤ m): 
             pureBeyond clauses index bound parity m := by
                   intro k
@@ -266,12 +302,12 @@ def pureBeyondVacuous{dom n : Nat}(clauses : FinSeq dom  (Clause n))
                   exact (False.elim (Nat.ltIrrefl k inq2))
                   done
 
-structure IsPureVarBeyond{dom n : Nat}(clauses : FinSeq dom  (Clause n))
+structure IsPureVarBeyond{dom n : Nat}(clauses : Vector  (Clause n) dom)
                       (index: Nat)(bound : index < n)(parity : Bool)(m: Nat) where
   evidence : pureBeyond clauses index bound parity m
 
 def varIsPureRec{n : Nat}(index: Nat)(bound : index < n)(parity : Bool) : 
-  (dom: Nat) →  (clauses : FinSeq dom  (Clause n)) → 
+  (dom: Nat) →  (clauses : Vector  (Clause n) dom) → 
     (m: Nat) → Option (IsPureVarBeyond clauses index bound parity m) →
     Option (IsPureVar clauses index bound parity) :=
     fun dom clauses m =>
@@ -284,7 +320,7 @@ def varIsPureRec{n : Nat}(index: Nat)(bound : index < n)(parity : Bool) :
         | none => none
         | some pureBeyondEv => 
           if pw : p < dom then
-            let head := clauses p pw index bound
+            let head := Vector.at (clauses.at p pw) index bound
               if pf : (head = none) ∨  (head = some parity) then
                 let evidence : pureBeyond clauses index bound parity p := 
                   by
@@ -293,7 +329,7 @@ def varIsPureRec{n : Nat}(index: Nat)(bound : index < n)(parity : Bool) :
                     intro ineq
                     cases Nat.eqOrLtOfLe ineq with
                     | inl eql =>           
-                      let lem1 : clauses p pw = clauses k kw := by
+                      let lem1 : clauses.at p pw = clauses.at k kw := by
                         apply witnessIndependent
                         exact eql
                         done
@@ -309,13 +345,13 @@ def varIsPureRec{n : Nat}(index: Nat)(bound : index < n)(parity : Bool) :
             none -- can recurse here but never called so making TCO easy
 
 def varIsPure{n : Nat}(index: Nat)(bound : index < n)(parity : Bool) : 
-  (dom: Nat) →  (clauses : FinSeq dom  (Clause n)) → 
+  (dom: Nat) →  (clauses : Vector  (Clause n) dom) → 
     Option (IsPureVar clauses index bound parity) :=
     fun dom clauses =>
       varIsPureRec index bound parity dom clauses dom 
         (some ⟨pureBeyondVacuous clauses index bound parity dom (Nat.leRefl _)⟩)
 
-def findPureAux{n : Nat} : (dom: Nat) →  (clauses : FinSeq dom (Clause (n +1))) → 
+def findPureAux{n : Nat} : (dom: Nat) →  (clauses : Vector  (Clause (n +1)) dom) → 
   (ub: Nat) → (lt : ub < n + 1) → 
       Option (HasPureVar clauses) :=
       fun dom clauses ub => 
@@ -348,7 +384,7 @@ def findPureAux{n : Nat} : (dom: Nat) →  (clauses : FinSeq dom (Clause (n +1))
             |none =>
               findPureAux dom clauses l (leStep lt)
             
-def hasPure{n : Nat}{dom: Nat}(clauses : FinSeq dom  (Clause (n +1))) 
+def hasPure{n : Nat}{dom: Nat}(clauses : Vector  (Clause (n +1)) dom) 
              : Option (HasPureVar clauses) :=
           findPureAux dom clauses n (Nat.leRefl _)
 
